theories/operations.v
@@ -64,11 +64,11 @@ Definition mem_size (m : memory) : N :=
   * @param len_delta: the number of bytes to grow the memory by
   *)
 Definition mem_grow (m : memory) (len_delta : N) : option memory :=
-  let new_length := N.add (mem_length m) len_delta in
-  let new_mem_data := mem_grow len_delta m.(mem_data) in
+  let new_size := N.add (mem_size m) len_delta in
+  let new_mem_data := mem_grow (N.mul len_delta page_size) m.(mem_data) in
   match m.(mem_max_opt) with
   | Some maxlim =>
-    if N.leb new_length maxlim then
+    if N.leb new_size maxlim then
       Some {|
         mem_data := new_mem_data;
         mem_max_opt := m.(mem_max_opt);
